interface for Record

src/tls/Record.fst
@@ -17,114 +17,10 @@ open Content
 module HS = FStar.HyperStack
 module ST = FStar.HyperStack.ST
 
-// Consider merging some of this module with Content?
-
-(* A flag for runtime debugging of record data.
-   The F* normalizer will erase debug prints at extraction
-   when this flag is set to false. *)
-private val discard: bool -> ST unit
-  (requires (fun _ -> True))
-  (ensures (fun h0 _ h1 -> h0 == h1))
-private let discard _ = ()
-private let print s = discard (IO.debug_print_string ("REC| "^s^"\n"))
-private unfold val trace: s:string -> ST unit
-  (requires (fun _ -> True))
-  (ensures (fun h0 _ h1 -> h0 == h1))
-private unfold let trace = if DebugFlags.debug_Record then print else (fun _ -> ())
-
-
-private let p_of_f (f:bytes): (p:FStar.Bytes.bytes{ FStar.Bytes.length p = FStar.Bytes.length f }) = f
-private let f_of_p (p:FStar.Bytes.bytes): (f:bytes{ FStar.Bytes.length p = FStar.Bytes.length f }) = p
-private let ctBytes x = f_of_p (ctBytes x)
-private let parseCT (x: lbytes 1) = parseCT (p_of_f x)
-private let versionBytes x = f_of_p (versionBytes x) 
-private let parseVersion (x: lbytes 2) = parseVersion (p_of_f x)
-
-
-// ------------------------outer packet format -------------------------------
-
-// the "outer" header has the same format for all versions of TLS
-// but TLS 1.3 fakes its content type and protocol version.
-
-private let headerLen = 5ul 
-private (* noextract *) let headerLength = v headerLen 
-private type header = b:lbytes headerLength // for all TLS versions
-
 #reset-options "--using_facts_from '* -LowParse.Spec.Base'"
 
-private let fake = ctBytes Application_data @| versionBytes TLS_1p2
-
-// this is the outer packet; to comply with legacy version signalling,
-// the *caller* should switch from 1.3 to 1.0 whenever data is
-// encrypted.
 #set-options "--z3rlimit 10" //18-04-20 now required; why?
-private inline_for_extraction 
-let makeHeader ct plain ver (length:nat {repr_bytes length <= 2}): header =
-  let ct_ver = 
-    if TLS_1p3? ver then if plain then 
-      (ctBytes ct @| versionBytes TLS_1p2) 
-    else 
-      fake 
-    else 
-      (ctBytes ct @| versionBytes ver) in
-  ct_ver @| bytes_of_int 2 length 
-
-// used only for testing
-let makePacket ct plain ver (data: (b:bytes { repr_bytes (length b) <= 2})) =
-  makeHeader ct plain ver (length data) @| data
-
-let sendPacket tcp ct plain ver (data: (b:bytes { repr_bytes (length b) <= 2})) =
-  // still some margin for progress to avoid intermediate copies
-  let header = makeHeader ct plain ver (length data) in 
-  trace ("record headers: "^print_bytes header);
-  let res = Transport.send tcp (BufferBytes.from_bytes header) headerLen in
-  if res = Int.Cast.uint32_to_int32 headerLen then 
-    let res = Transport.send tcp (BufferBytes.from_bytes data) (len data) in
-    if Int32.v res = length data
-    then Correct()
-    else Error(Printf.sprintf "Transport.send(header) returned %l" res)
-  else   Error(Printf.sprintf "Transport.send(payload) returned %l" res)
-
-private type parsed_header = result (contentType
-                           * protocolVersion
-                           * l:nat { l <= max_TLSCiphertext_fragment_length})
-// private // QUIC.fst needs access to this definition
-val parseHeader: h5:header -> Tot parsed_header
-
-let parseHeader (h5:header) =
-    let (ct1,b4)   = FStar.Bytes.split h5 1ul in
-    let (pv2,len2) = FStar.Bytes.split b4 2ul in
-    match parseCT ct1 with
-    | Error z -> Error z
-    | Correct ct ->
-      match parseVersion pv2 with
-      | Error z -> Error z
-      | Correct (Unknown_protocolVersion _) ->
-        fatal Decode_error (perror __SOURCE_FILE__ __LINE__ "Parsed unknown protocol version")
-      | Correct pv ->
-          let len = int_of_bytes len2 in
-          if len <= 0 || len > max_TLSCiphertext_fragment_length
-          then fatal Illegal_parameter (perror __SOURCE_FILE__ __LINE__ "Wrong fragment length")
-          else correct(ct,pv,len)
-
-
-(*** networking ***)
-
-// in the spirit of TLS 1.3, we ignore the outer protocol version (see appendix C):
-// our server never treats the ClientHello's record pv as its minimum supported pv;
-// our client never checks the consistency of the server's record pv.
-// (see earlier versions for the checks we used to perform)
-
-// connectlon-local input state
-type partial =
-  | Header
-  | Body: ct: contentType -> pv: protocolVersion -> partial
-
-private let maxlen = headerLen +^ UInt32.uint_to_t max_TLSCiphertext_fragment_length
-private type input_buffer = b: Buffer.buffer UInt8.t {Buffer.length b = v maxlen}
-
-//TODO index by region. // number of bytes already buffered
-noeq abstract type input_state = | InputState:
+noeq type input_state = | InputState:
   pos: ref (len:UInt32.t {len <=^ maxlen}) ->
   b: input_buffer {
     Buffer.disjoint_ref_1 b pos /\
@@ -132,14 +28,7 @@ noeq abstract type input_state = | InputState:
     Buffer.length b = v maxlen} -> 
   input_state
 
-private let parseHeaderBuffer (b: Buffer.buffer UInt8.t {Buffer.length b = headerLength}) : ST parsed_header
-  (requires (fun h0 -> Buffer.live h0 b))
-  (ensures (fun h0 hdr h1 -> h0 == h1 /\ hdr = parseHeader (Bytes.hide (Buffer.as_seq h0 b))))
-=
-  // some margin for progress
-  parseHeader (BufferBytes.to_bytes headerLength b)
-
-abstract let input_inv h0 (s: input_state) = 
+let input_inv h0 (s: input_state) = 
   Mem.contains h0 s.pos /\
   Buffer.live h0 s.b /\
   ( let p0 = UInt32.v (sel h0 s.pos) in 
@@ -150,17 +39,8 @@ abstract let input_inv h0 (s: input_state) =
       | _                    -> False ))
 // we are waiting either for header bytes or payload bytes
 
-private unfold val waiting_len:  s: input_state -> ST UInt32.t
-  (requires fun h0 -> input_inv h0 s)
-  (ensures fun h0 len h1 -> 
-    h0 == h1 /\
-    ( let pv = UInt32.v (sel h0 s.pos) in 
-      let l = UInt32.v len in 
-      ( if pv < headerLength 
-        then pv + l = headerLength
-        else 
-        match parseHeader (Bytes.hide (Buffer.as_seq h0 (Buffer.sub s.b 0ul headerLen))) with
-        | Correct (_,_,length) -> pv + l == headerLength + length)))
+let input_pos s = s.pos
+let input_b s = s.b
 
 #reset-options "--max_fuel 0 --max_ifuel 0 --using_facts_from '* -LowParse -Format'"
 let waiting_len s =
@@ -172,41 +52,10 @@ let waiting_len s =
 
 // TODO later, use a length-field accessor instead of a header parser
 
-val alloc_input_state: r:_ -> ST input_state 
-  (requires (fun h0 -> is_eternal_region r))
-  (ensures (fun h0 s h1 ->
-    //18-04-20 TODO post-condition for allocating a ref and a buffer?
-    Mem.frameOf s.pos = r /\ 
-    input_inv h1 s))
 let alloc_input_state r = 
   let pos = ralloc r 0ul in
   let b = Buffer.rcreate r 0uy maxlen in
   InputState pos b
-
-type read_result =
-  | ReadError of TLSError.error
-  | ReadWouldBlock
-  | Received:
-      ct:contentType ->
-      pv:protocolVersion ->
-      b:bytes {length b <= max_TLSCiphertext_fragment_length} -> read_result
-
-// 2018.04.25 SZ:
-// I had to modify the post-condition to say `input_inv` is preserved only if
-// the result is not a ReadError.
-// We return a ReadError when the header is invalid, but we still advance s.pos.
-// We could preserve the invariant unconditionally if we advanced it only when
-// the header is valid.
-val read: Transport.t -> s: input_state -> ST read_result
-  (requires fun h0 -> input_inv h0 s)
-  (ensures fun h0 r h1 -> ReadError? r \/ input_inv h1 s)
-//18-04-20 TODO modifies clause on a ref + a buffer
-// let r = Mem.frameOf s.pos in
-// Mem.modifies_one r h0 h1 
-// Buffer.modifies_bufs_and_refs
-//   (Buffer.only s.b)
-//   (Set.singleton (Heap.addr_of (HS.as_ref s.pos)))
-//   h0 h1)
 
 #reset-options "--max_fuel 0 --max_ifuel 0 --using_facts_from '* -LowParse -Format' --z3rlimit 30"
 let rec read tcp s =
