src/tls/Record.fsti
@@ -1,0 +1,212 @@
+module Record
+
+(* (optional) encryption and processing of the outer, untrusted record format *)
+
+open FStar.Seq
+open FStar.Bytes
+open FStar.Error
+open FStar.UInt32
+
+open Mem
+open TLSError
+open TLSInfo
+open TLSConstants
+open Range
+open Content
+
+module HS = FStar.HyperStack
+module ST = FStar.HyperStack.ST
+
+// Consider merging some of this module with Content?
+
+(* A flag for runtime debugging of record data.
+   The F* normalizer will erase debug prints at extraction
+   when this flag is set to false. *)
+private let discard (_:bool) : ST unit
+  (requires (fun _ -> True))
+  (ensures (fun h0 _ h1 -> h0 == h1)) = ()
+private let print s = discard (IO.debug_print_string ("REC| "^s^"\n"))
+private unfold let trace: s:string -> ST unit
+  (requires (fun _ -> True))
+  (ensures (fun h0 _ h1 -> h0 == h1)) =
+  if DebugFlags.debug_Record then print else (fun _ -> ())
+
+
+private let p_of_f (f:bytes): (p:FStar.Bytes.bytes{ FStar.Bytes.length p = FStar.Bytes.length f }) = f
+private let f_of_p (p:FStar.Bytes.bytes): (f:bytes{ FStar.Bytes.length p = FStar.Bytes.length f }) = p
+private let ctBytes x = f_of_p (ctBytes x)
+private let parseCT (x: lbytes 1) = parseCT (p_of_f x)
+private let versionBytes x = f_of_p (versionBytes x) 
+private let parseVersion (x: lbytes 2) = parseVersion (p_of_f x)
+
+
+// ------------------------outer packet format -------------------------------
+
+// the "outer" header has the same format for all versions of TLS
+// but TLS 1.3 fakes its content type and protocol version.
+
+private let headerLen = 5ul 
+private (* noextract *) let headerLength = v headerLen 
+private type header = b:lbytes headerLength // for all TLS versions
+
+#reset-options "--using_facts_from '* -LowParse.Spec.Base'"
+
+private let fake = ctBytes Application_data @| versionBytes TLS_1p2
+
+// this is the outer packet; to comply with legacy version signalling,
+// the *caller* should switch from 1.3 to 1.0 whenever data is
+// encrypted.
+#set-options "--z3rlimit 10" //18-04-20 now required; why?
+private inline_for_extraction 
+let makeHeader ct plain ver (length:nat {repr_bytes length <= 2}): header =
+  let ct_ver = 
+    if TLS_1p3? ver then if plain then 
+      (ctBytes ct @| versionBytes TLS_1p2) 
+    else 
+      fake 
+    else 
+      (ctBytes ct @| versionBytes ver) in
+  ct_ver @| bytes_of_int 2 length 
+
+// used only for testing
+let makePacket ct plain ver (data: (b:bytes { repr_bytes (length b) <= 2})) =
+  makeHeader ct plain ver (length data) @| data
+
+let sendPacket tcp ct plain ver (data: (b:bytes { repr_bytes (length b) <= 2})) =
+  // still some margin for progress to avoid intermediate copies
+  let header = makeHeader ct plain ver (length data) in 
+  trace ("record headers: "^print_bytes header);
+  let res = Transport.send tcp (BufferBytes.from_bytes header) headerLen in
+  if res = Int.Cast.uint32_to_int32 headerLen then 
+    let res = Transport.send tcp (BufferBytes.from_bytes data) (len data) in
+    if Int32.v res = length data
+    then Correct()
+    else Error(Printf.sprintf "Transport.send(header) returned %l" res)
+  else   Error(Printf.sprintf "Transport.send(payload) returned %l" res)
+
+private type parsed_header = result (contentType
+                           * protocolVersion
+                           * l:nat { l <= max_TLSCiphertext_fragment_length})
+// private // QUIC.fst needs access to this definition
+let parseHeader (h5:header) : Tot parsed_header =
+    let (ct1,b4)   = FStar.Bytes.split h5 1ul in
+    let (pv2,len2) = FStar.Bytes.split b4 2ul in
+    match parseCT ct1 with
+    | Error z -> Error z
+    | Correct ct ->
+      match parseVersion pv2 with
+      | Error z -> Error z
+      | Correct (Unknown_protocolVersion _) ->
+        fatal Decode_error (perror __SOURCE_FILE__ __LINE__ "Parsed unknown protocol version")
+      | Correct pv ->
+          let len = int_of_bytes len2 in
+          if len <= 0 || len > max_TLSCiphertext_fragment_length
+          then fatal Illegal_parameter (perror __SOURCE_FILE__ __LINE__ "Wrong fragment length")
+          else correct(ct,pv,len)
+
+
+(*** networking ***)
+
+// in the spirit of TLS 1.3, we ignore the outer protocol version (see appendix C):
+// our server never treats the ClientHello's record pv as its minimum supported pv;
+// our client never checks the consistency of the server's record pv.
+// (see earlier versions for the checks we used to perform)
+
+// connectlon-local input state
+type partial =
+  | Header
+  | Body: ct: contentType -> pv: protocolVersion -> partial
+
+private let maxlen = headerLen +^ UInt32.uint_to_t max_TLSCiphertext_fragment_length
+private type input_buffer = b: Buffer.buffer UInt8.t {Buffer.length b = v maxlen}
+
+//TODO index by region. // number of bytes already buffered
+val input_state : Type0
+
+private let parseHeaderBuffer (b: Buffer.buffer UInt8.t {Buffer.length b = headerLength}) : ST parsed_header
+  (requires (fun h0 -> Buffer.live h0 b))
+  (ensures (fun h0 hdr h1 -> h0 == h1 /\ hdr = parseHeader (Bytes.hide (Buffer.as_seq h0 b))))
+=
+  // some margin for progress
+  parseHeader (BufferBytes.to_bytes headerLength b)
+
+val input_inv (h0:HS.mem) (s: input_state) : Type0
+
+val input_pos (s:input_state) : Tot (ref (len:UInt32.t{len <=^ maxlen}))
+
+val input_b (s:input_state)
+: Tot (b: input_buffer{
+          Buffer.disjoint_ref_1 b (input_pos s) /\
+          Buffer.frameOf b = Mem.frameOf (input_pos s) /\ 
+          Buffer.length b = v maxlen})
+
+
+// we are waiting either for header bytes or payload bytes
+
+private val waiting_len:  s: input_state -> ST UInt32.t
+  (requires fun h0 -> input_inv h0 s)
+  (ensures fun h0 len h1 -> 
+    h0 == h1 /\
+    ( let pv = UInt32.v (sel h0 (input_pos s)) in 
+      let l = UInt32.v len in 
+      ( if pv < headerLength 
+        then pv + l = headerLength
+        else 
+        match parseHeader (Bytes.hide (Buffer.as_seq h0 (Buffer.sub (input_b s) 0ul headerLen))) with
+        | Correct (_,_,length) -> pv + l == headerLength + length
+        | _ -> False)))
+
+// TODO later, use a length-field accessor instead of a header parser
+
+val alloc_input_state: r:_ -> ST input_state 
+  (requires (fun h0 -> is_eternal_region r))
+  (ensures (fun h0 s h1 ->
+    //18-04-20 TODO post-condition for allocating a ref and a buffer?
+    Mem.frameOf (input_pos s) = r /\ 
+    input_inv h1 s))
+
+type read_result =
+  | ReadError of TLSError.error
+  | ReadWouldBlock
+  | Received:
+      ct:contentType ->
+      pv:protocolVersion ->
+      b:bytes {length b <= max_TLSCiphertext_fragment_length} -> read_result
+
+// 2018.04.25 SZ:
+// I had to modify the post-condition to say `input_inv` is preserved only if
+// the result is not a ReadError.
+// We return a ReadError when the header is invalid, but we still advance s.pos.
+// We could preserve the invariant unconditionally if we advanced it only when
+// the header is valid.
+val read: Transport.t -> s: input_state -> ST read_result
+  (requires fun h0 -> input_inv h0 s)
+  (ensures fun h0 r h1 -> ReadError? r \/ input_inv h1 s)
+//18-04-20 TODO modifies clause on a ref + a buffer
+// let r = Mem.frameOf s.pos in
+// Mem.modifies_one r h0 h1 
+// Buffer.modifies_bufs_and_refs
+//   (Buffer.only s.b)
+//   (Set.singleton (Heap.addr_of (HS.as_ref s.pos)))
+//   h0 h1)
+
+(*        
+//18-01-24 recheck async 
+//    if length fresh = 0 then
+//      ReadError(AD_internal_error,"TCP close") // otherwise we loop...
+
+assert( Mem.contains h2 s.pos /\ Buffer.live h2 s.b )
+
+assert(
+  if v p0 < headerLength 
+  then v p1 = headerLength 
+  else 
+    match parseHeader (Bytes.hide (Buffer.as_seq h0 (Buffer.sub s.b 0ul headerLen))) with
+    | Correct (_,_,length) -> v p1 = headerLength + length 
+    | _                    -> False)
+
+assert(
+  match parseHeader (Bytes.hide (Buffer.as_seq h1 (Buffer.sub s.b 0ul headerLen))) with
+  | Correct (_,_,length) -> v p1 = headerLength + length 
+  | _                    -> False)
+*)
